tune ty_own simplification behavior; make uninit.(ty_own) compute the right way

theories/typing/uninit.v
@@ -19,13 +19,32 @@ Section uninit.
   Lemma uninit0_sz n : ty_size (uninit0 n) = n.
   Proof. induction n=>//=. by f_equal. Qed.
 
-  (* We redefine uninit as an alias of uninit0, so that the size
-     computes directly to [n] *)
+  Lemma uninit0_own n tid vl :
+    ty_own (uninit0 n) tid vl ⊣⊢ ⌜length vl = n⌝.
+  Proof.
+    iSplit.
+    - iIntros "Hvl".
+      iInduction n as [|n] "IH" forall (vl); simpl.
+      + iDestruct "Hvl" as "%". subst vl. done.
+      + iDestruct "Hvl" as (vl1 vl2) "(% & % & Hprod)".
+        destruct vl1 as [|v [|]]; try done. subst vl. simpl.
+        iDestruct ("IH" with "Hprod") as "%". iPureIntro. by f_equal.
+    - iIntros "%". subst n. iInduction vl as [|v vl] "IH"; first done.
+      simpl. iExists [v], vl. auto.
+  Qed.
+
+  (* We redefine uninit as an alias of uninit0, so that ty_size and ty_own
+     compute directly.  We re-use the sharing from the product as that saves a whole
+     lot of work. *)
   Program Definition uninit (n : nat) : type :=
-    {| ty_size := n; ty_own := (uninit0 n).(ty_own);
+    {| ty_size := n; ty_own tid vl := ⌜length vl = n⌝%I;
        ty_shr := (uninit0 n).(ty_shr) |}.
-  Next Obligation. intros. by rewrite ty_size_eq uninit0_sz. Qed.
-  Next Obligation. intros. by apply ty_share. Qed.
+  Next Obligation. iIntros (???) "%". done. Qed.
+  Next Obligation.
+    iIntros (???????) "LFT Hvl". iApply (ty_share (uninit0 n) with "LFT"); first done.
+    iApply (bor_iff with "[] Hvl"). iIntros "!> !#". setoid_rewrite uninit0_own.
+    iSplit; iIntros; done.
+  Qed.
   Next Obligation. intros. by apply ty_shr_mono. Qed.
 
   Global Instance uninit_wf n : TyWf (uninit n) :=
@@ -33,22 +52,32 @@ Section uninit.
 
   Global Instance uninit_copy n : Copy (uninit n).
   Proof.
-    destruct (product_copy (replicate n uninit_1)) as [A B].
-      by apply Forall_replicate, _.
-    rewrite uninit0_sz in B. by split.
+    assert (Copy (uninit0 n)) as [A B].
+    { apply product_copy. by apply Forall_replicate, _. }
+    split; first by apply _.
+    rewrite uninit0_sz in B. setoid_rewrite uninit0_own in B. done.
   Qed.
 
   Global Instance uninit_send n : Send (uninit n).
-  Proof. apply product_send, Forall_replicate, _. Qed.
+  Proof. iIntros (???) "?". done. Qed.
 
   Global Instance uninit_sync n : Sync (uninit n).
   Proof. apply product_sync, Forall_replicate, _. Qed.
 
+  (* Unfolding lemma, kep only for backwards compatibility. *)
+  Lemma uninit_own n tid vl :
+    (uninit n).(ty_own) tid vl ⊣⊢ ⌜length vl = n⌝.
+  Proof. done. Qed.
+
   Lemma uninit_uninit0_eqtype E L n :
     eqtype E L (uninit0 n) (uninit n).
-  Proof. apply equiv_eqtype; constructor=>//=. apply uninit0_sz. Qed.
+  Proof.
+    apply equiv_eqtype; constructor=>//=.
+    - apply uninit0_sz.
+    - iIntros (??). rewrite uninit0_own. done.
+  Qed.
 
-  Lemma uninit_product_subtype_cons {E L} (n : nat) ty tyl :
+  Lemma uninit_product_subtype_cons_r {E L} (n : nat) ty tyl :
     ty.(ty_size) ≤ n →
     subtype E L (uninit ty.(ty_size)) ty →
     subtype E L (uninit (n-ty.(ty_size))) (Π tyl) →
@@ -58,7 +87,7 @@ Section uninit.
     rewrite (le_plus_minus ty.(ty_size) n) // replicate_plus
            -(prod_flatten_r _ _ [_]) /= -prod_app. repeat (done || f_equiv).
   Qed.
-  Lemma uninit_product_subtype_cons' {E L} (n : nat) ty tyl :
+  Lemma uninit_product_subtype_cons_l {E L} (n : nat) ty tyl :
     ty.(ty_size) ≤ n →
     subtype E L ty (uninit ty.(ty_size)) →
     subtype E L (Π tyl) (uninit (n-ty.(ty_size))) →
@@ -68,22 +97,22 @@ Section uninit.
     rewrite (le_plus_minus ty.(ty_size) n) // replicate_plus
            -(prod_flatten_r _ _ [_]) /= -prod_app. repeat (done || f_equiv).
   Qed.
-  Lemma uninit_product_eqtype_cons {E L} (n : nat) ty tyl :
+  Lemma uninit_product_eqtype_cons_r {E L} (n : nat) ty tyl :
     ty.(ty_size) ≤ n →
     eqtype E L (uninit ty.(ty_size)) ty →
     eqtype E L (uninit (n-ty.(ty_size))) (Π tyl) →
     eqtype E L (uninit n) (Π(ty :: tyl)).
   Proof.
     intros ? [] []. split.
-    - by apply uninit_product_subtype_cons.
-    - by apply uninit_product_subtype_cons'.
+    - by apply uninit_product_subtype_cons_r.
+    - by apply uninit_product_subtype_cons_l.
   Qed.
-  Lemma uninit_product_eqtype_cons' {E L} (n : nat) ty tyl :
+  Lemma uninit_product_eqtype_cons_l {E L} (n : nat) ty tyl :
     ty.(ty_size) ≤ n →
     eqtype E L ty (uninit ty.(ty_size)) →
     eqtype E L (Π tyl) (uninit (n-ty.(ty_size))) →
     eqtype E L (Π(ty :: tyl)) (uninit n).
-  Proof. symmetry. by apply uninit_product_eqtype_cons. Qed.
+  Proof. symmetry. by apply uninit_product_eqtype_cons_r. Qed.
 
   Lemma uninit_unit_eqtype E L n :
     n = 0%nat →
@@ -101,21 +130,9 @@ Section uninit.
     n = 0%nat →
     subtype E L unit (uninit n).
   Proof. rewrite -uninit_uninit0_eqtype=>->//. Qed.
-
-  Lemma uninit_own n tid vl :
-    (uninit n).(ty_own) tid vl ⊣⊢ ⌜length vl = n⌝.
-  Proof.
-    iSplit.
-    - rewrite ty_size_eq. auto.
-    - iInduction vl as [|v vl] "IH" forall (n).
-      + iIntros "%". by destruct n; simpl.
-      + iIntros (Heq). destruct n; first done. simpl.
-        iExists [v], vl. iSplit; first done. iSplit; first done.
-        unfold uninit0, product. iApply "IH". by inversion Heq.
-  Qed.
 End uninit.
 
-Hint Resolve uninit_product_eqtype_cons uninit_product_eqtype_cons'
-             uninit_product_subtype_cons uninit_product_subtype_cons'
+Hint Resolve uninit_product_eqtype_cons_l uninit_product_eqtype_cons_r
+             uninit_product_subtype_cons_l uninit_product_subtype_cons_r
              uninit_unit_eqtype uninit_unit_eqtype'
              uninit_unit_subtype uninit_unit_subtype' : lrust_typing.
